Trabalhando no contrato da classe. Sem implementação

Queue.dfy
@@ -1,21 +1,44 @@
-class Queue {
-    // Atributos
+class {:autocontracts} Queue {
+      // Atributos
+  var circularQueue: array<int>;
+  var rear: int;
+  var front: int;
 
-    var circularQueue: array<int>;
-    var rear: int;
-    var front: int;
-    var maxSize: int;
+  // Abstração
+  ghost var Content: seq<int>;
+
+  // Predicado
+  ghost predicate Valid()
+    {
+    
+    }
 
     // Construtor
-
     constructor()
+      ensures Content == []
+    {
+    circularQueue := new int[0];
+    rear := 0;
+    front := 0;
+    Content := [];
+    }
 
-    // Métodos
+  // Métodos
 
-    method insert()
-    method remove()
-    method contains()
-    method size()
-    method isEmpty()
-    method mergeQueues()
+  method insert(item: int)
+    ensures Content == old(Content) + [item]
+
+  method remove(item: int)
+    requires |Content| > 0
+    ensures item == old(Content)[0]
+    ensures Content == old(Content)[1..]
+
+  method size() returns (size:nat)
+    ensures size == |Content|
+    ensures Content == old(Content)
+
+  // TODO
+  // method contains()
+  // method isEmpty() returns (isEmpty:bool)
+  // method mergeQueues() returns (mergedQueue:array<int>)
 }
